MMU_ARMv7_Refinement_No_Fault/ARMv7_Flush_Ref.thy
@@ -18,28 +18,28 @@ lemma flush_tlb_non_det_det_refine:
   by (cases s, cases t , clarsimp simp: state.defs tlb_rel_def) 
 
 
-lemma  flush_tlb_det_sat_no_flt_refine:
-  "\<lbrakk> Flush_TLB (s::tlb_det_state) = ((), s') ;  Flush_TLB(t::tlb_sat_no_flt_state) = ((), t'); 
-         tlb_rel_sat_no_flt (typ_det_tlb s) (typ_sat_no_flt_tlb t) \<rbrakk> \<Longrightarrow> 
-                  tlb_rel_sat_no_flt (typ_det_tlb s') (typ_sat_no_flt_tlb t')"
-  apply (clarsimp simp: Flush_TLB_tlb_det_state_ext_def Flush_TLB_tlb_sat_no_flt_state_ext_def)
-  apply (clarsimp simp: tlb_rel_sat_no_flt_def saturated_no_flt_def)
+lemma  flush_tlb_det_sat_refine:
+  "\<lbrakk> Flush_TLB (s::tlb_det_state) = ((), s') ;  Flush_TLB(t::tlb_sat_state) = ((), t'); 
+         tlb_rel_sat (typ_det_tlb s) (typ_sat_tlb t) \<rbrakk> \<Longrightarrow> 
+                  tlb_rel_sat (typ_det_tlb s') (typ_sat_tlb t')"
+  apply (clarsimp simp: Flush_TLB_tlb_det_state_ext_def Flush_TLB_tlb_sat_state_ext_def)
+  apply (clarsimp simp: tlb_rel_sat_def saturated_def)
   apply (cases s, cases t , clarsimp simp: state.defs)
   done
 
 
-lemma flush_tlb_sat_no_flt_abs_refine':
-  "\<lbrakk>Flush_TLB (s::tlb_sat_no_flt_state) = ((), s') ;  Flush_TLB (t::tlb_incon_state') = ((), t'); 
-             tlb_rel_abs' (typ_sat_no_flt_tlb s) (typ_incon' t) \<rbrakk> \<Longrightarrow> 
-                     tlb_rel_abs' (typ_sat_no_flt_tlb s') (typ_incon' t')"
-  apply (clarsimp simp: Flush_TLB_tlb_sat_no_flt_state_ext_def
+lemma flush_tlb_sat_abs_refine':
+  "\<lbrakk>Flush_TLB (s::tlb_sat_state) = ((), s') ;  Flush_TLB (t::tlb_incon_state') = ((), t'); 
+             tlb_rel_abs' (typ_sat_tlb s) (typ_incon' t) \<rbrakk> \<Longrightarrow> 
+                     tlb_rel_abs' (typ_sat_tlb s') (typ_incon' t')"
+  apply (clarsimp simp: Flush_TLB_tlb_sat_state_ext_def
       Flush_TLB_tlb_incon_state'_ext_def tlb_rel_abs'_def)
   apply (rule conjI)
    apply (cases s, cases t, clarsimp simp: state.defs)
   apply (rule conjI)
    apply (clarsimp simp: asid_va_incon_tlb_mem_def)
    apply (rule conjI)
-    apply (clarsimp simp: asid_va_incon_def lookup_no_flt_range_pt_walk_not_incon')
+    apply (clarsimp simp: asid_va_incon_def lookup_range_pt_walk_not_incon')
    apply (clarsimp simp: asid_va_hit_incon_inter_def)
    apply (rule conjI)
     apply (clarsimp simp: asid_va_hit_incon'_def)
@@ -49,7 +49,7 @@ lemma flush_tlb_sat_no_flt_abs_refine':
     apply clarsimp
    apply (clarsimp simp: asid_va_hit_incon''_def lookup_miss_is_fault_intro)
   apply (rule conjI)
-   apply (clarsimp simp: saturated_no_flt_def)
+   apply (clarsimp simp: saturated_def)
   apply (clarsimp simp: snapshot_of_tlb_def asid_unequal_miss'')
   done
 
@@ -74,12 +74,12 @@ lemma flush_asid_non_det_det_refine:
   apply (cases s, cases t , clarsimp simp: state.defs tlb_rel_def) 
   by blast
 
-lemma  flush_asid_det_sat_no_flt_refine:
-  "\<lbrakk> Flush_ASID a (s::tlb_det_state) = ((), s') ;  Flush_ASID a (t::tlb_sat_no_flt_state) = ((), t'); 
-         tlb_rel_sat_no_flt (typ_det_tlb s) (typ_sat_no_flt_tlb t) \<rbrakk> \<Longrightarrow> 
-                  tlb_rel_sat_no_flt (typ_det_tlb s') (typ_sat_no_flt_tlb t')"
-  apply (clarsimp simp: Flush_ASID_tlb_det_state_ext_def Flush_ASID_tlb_sat_no_flt_state_ext_def)
-  apply (clarsimp simp: tlb_rel_sat_no_flt_def saturated_no_flt_def)
+lemma  flush_asid_det_sat_refine:
+  "\<lbrakk> Flush_ASID a (s::tlb_det_state) = ((), s') ;  Flush_ASID a (t::tlb_sat_state) = ((), t'); 
+         tlb_rel_sat (typ_det_tlb s) (typ_sat_tlb t) \<rbrakk> \<Longrightarrow> 
+                  tlb_rel_sat (typ_det_tlb s') (typ_sat_tlb t')"
+  apply (clarsimp simp: Flush_ASID_tlb_det_state_ext_def Flush_ASID_tlb_sat_state_ext_def)
+  apply (clarsimp simp: tlb_rel_sat_def saturated_def)
   apply (cases s, cases t , clarsimp simp: state.defs)
   by blast
 
@@ -105,8 +105,8 @@ lemma  lookup_asid_hit_diff:
 
  
 lemma  lookup_minus_hit_asid_hit:
-  "\<lbrakk>lookup (tlb_sat_no_flt_set s - {e \<in> tlb_sat_no_flt_set s. asid_entry e = a}) a' va = Hit x; a \<noteq> a'\<rbrakk> \<Longrightarrow> 
-                         lookup (tlb_sat_no_flt_set s) a' va = Hit x"
+  "\<lbrakk>lookup (tlb_sat_set s - {e \<in> tlb_sat_set s. asid_entry e = a}) a' va = Hit x; a \<noteq> a'\<rbrakk> \<Longrightarrow> 
+                         lookup (tlb_sat_set s) a' va = Hit x"
   apply (clarsimp simp: lookup_def entry_set_def entry_range_asid_tags_def split: if_split_asm)
   apply safe
   by auto
@@ -122,20 +122,20 @@ lemma diff_asid_lookup_union:
   "\<lbrakk> a' \<noteq> a; a' \<noteq> a'';
        asid_entry ` the ` {e \<in> range (pt_walk a'' m r). \<not> is_fault e} = {a''}  \<or>
             asid_entry ` the ` {e \<in> range (pt_walk a'' m r). \<not> is_fault e} = {}\<rbrakk>  \<Longrightarrow> 
-                 lookup (tlb_sat_no_flt_set s - {e \<in> tlb_sat_no_flt_set s. asid_entry e = a} \<union>
+                 lookup (tlb_sat_set s - {e \<in> tlb_sat_set s. asid_entry e = a} \<union>
                         the ` {e \<in> range (pt_walk a'' m r). \<not> is_fault e}) a' va =
-                                lookup (tlb_sat_no_flt_set s) a' va"
+                                lookup (tlb_sat_set s) a' va"
   apply (erule disjE)
-   apply (cases "lookup (tlb_sat_no_flt_set s - {e \<in> tlb_sat_no_flt_set s. asid_entry e = a} \<union>
+   apply (cases "lookup (tlb_sat_set s - {e \<in> tlb_sat_set s. asid_entry e = a} \<union>
                  the ` {e \<in> range (pt_walk a'' m r). \<not> is_fault e}) a' va" ; 
       (clarsimp simp: lookup_def entry_set_def entry_range_asid_tags_def split: if_split_asm , fastforce))
-  by (cases "lookup (tlb_sat_no_flt_set s - {e \<in> tlb_sat_no_flt_set s. asid_entry e = a} \<union>
+  by (cases "lookup (tlb_sat_set s - {e \<in> tlb_sat_set s. asid_entry e = a} \<union>
                  the ` {e \<in> range (pt_walk a'' m r). \<not> is_fault e})  a' va"; 
       (clarsimp simp: lookup_def entry_set_def entry_range_asid_tags_def split: if_split_asm , fastforce))
 
 lemma  asid_entry_set_inter:
   "a \<noteq> ASID s  \<Longrightarrow>   
-     {e \<in> tlb_sat_no_flt_set s. asid_entry e = a} \<inter> the ` {e \<in> range (pt_walk (ASID s) (MEM s) (TTBR0 s)). \<not> is_fault e} = {}"
+     {e \<in> tlb_sat_set s. asid_entry e = a} \<inter> the ` {e \<in> range (pt_walk (ASID s) (MEM s) (TTBR0 s)). \<not> is_fault e} = {}"
   apply (case_tac "{e \<in> range (pt_walk (ASID s) (MEM s) (TTBR0 s)). \<not> is_fault e} = {}")
    apply simp
    apply blast
@@ -151,13 +151,13 @@ lemma  asid_entry_set_inter:
 
 
 
-lemma flush_asid_sat_no_flt_abs_refine':
-  "\<lbrakk>Flush_ASID a (s::tlb_sat_no_flt_state) = ((), s') ;  Flush_ASID a (t::tlb_incon_state') = ((), t'); 
-             tlb_rel_abs' (typ_sat_no_flt_tlb s) (typ_incon' t) \<rbrakk> \<Longrightarrow> tlb_rel_abs' (typ_sat_no_flt_tlb s') (typ_incon' t')"
-  apply (clarsimp simp: Flush_ASID_tlb_sat_no_flt_state_ext_def Flush_ASID_tlb_incon_state'_ext_def tlb_rel_abs'_def)
+lemma flush_asid_sat_abs_refine':
+  "\<lbrakk>Flush_ASID a (s::tlb_sat_state) = ((), s') ;  Flush_ASID a (t::tlb_incon_state') = ((), t'); 
+             tlb_rel_abs' (typ_sat_tlb s) (typ_incon' t) \<rbrakk> \<Longrightarrow> tlb_rel_abs' (typ_sat_tlb s') (typ_incon' t')"
+  apply (clarsimp simp: Flush_ASID_tlb_sat_state_ext_def Flush_ASID_tlb_incon_state'_ext_def tlb_rel_abs'_def)
   apply (rule conjI)
    apply (cases s, cases t, clarsimp simp: state.defs)
-  apply (subgoal_tac "tlb_sat_no_flt_set s = tlb_sat_no_flt_set s \<union> 
+  apply (subgoal_tac "tlb_sat_set s = tlb_sat_set s \<union> 
                               the ` {e \<in> range (pt_walk (ASID s) (MEM s) (TTBR0 s)). \<not> is_fault e}")
    prefer 2
    apply (drule sat_state_tlb', clarsimp simp: state.defs)
@@ -166,9 +166,9 @@ lemma flush_asid_sat_no_flt_abs_refine':
    apply (rule conjI)
     apply (clarsimp simp: asid_va_incon_def)
     apply (case_tac "a \<noteq> ASID s")
-     apply (subgoal_tac "{e \<in> tlb_sat_no_flt_set s. asid_entry e = a} \<inter> the ` {e \<in> range (pt_walk (ASID s) (MEM s) (TTBR0 s)). \<not> is_fault e} = {}")
-      apply (subgoal_tac "tlb_sat_no_flt_set s - {e \<in> tlb_sat_no_flt_set s. asid_entry e = a} \<union> the ` {e \<in> range (pt_walk (ASID s) (MEM s) (TTBR0 s)). \<not> is_fault e} = 
-                     tlb_sat_no_flt_set s - {e \<in> tlb_sat_no_flt_set s. asid_entry e = a}")
+     apply (subgoal_tac "{e \<in> tlb_sat_set s. asid_entry e = a} \<inter> the ` {e \<in> range (pt_walk (ASID s) (MEM s) (TTBR0 s)). \<not> is_fault e} = {}")
+      apply (subgoal_tac "tlb_sat_set s - {e \<in> tlb_sat_set s. asid_entry e = a} \<union> the ` {e \<in> range (pt_walk (ASID s) (MEM s) (TTBR0 s)). \<not> is_fault e} = 
+                     tlb_sat_set s - {e \<in> tlb_sat_set s. asid_entry e = a}")
        prefer 2
        apply blast
       apply clarsimp
@@ -180,7 +180,7 @@ lemma flush_asid_sat_no_flt_abs_refine':
     apply clarsimp
     apply (drule union_incon_cases1)
     apply (erule disjE)
-     apply (clarsimp simp: lookup_no_flt_range_pt_walk_not_incon')
+     apply (clarsimp simp: lookup_range_pt_walk_not_incon')
     apply (erule disjE)
      apply clarsimp
      apply (subgoal_tac "aa \<noteq> ASID s")
@@ -199,7 +199,7 @@ lemma flush_asid_sat_no_flt_abs_refine':
      apply (drule lookup_incon_minus)
      apply blast
     apply (erule disjE)
-     apply (clarsimp simp: lookup_no_flt_range_pt_walk_not_incon')
+     apply (clarsimp simp: lookup_range_pt_walk_not_incon')
     apply clarsimp
     apply (rule conjI)
      prefer 2
@@ -209,13 +209,13 @@ lemma flush_asid_sat_no_flt_abs_refine':
    apply (clarsimp simp: asid_va_hit_incon_inter_def asid_va_hit_incon'_def)
    apply (rule conjI)
    apply (case_tac "a \<noteq> ASID s")
-    apply (subgoal_tac "{e \<in> tlb_sat_no_flt_set s. asid_entry e = a} \<inter> the ` {e \<in> range (pt_walk (ASID s) (MEM s) (TTBR0 s)). \<not> is_fault e} = {}")
-     apply (subgoal_tac "tlb_sat_no_flt_set s - {e \<in> tlb_sat_no_flt_set s. asid_entry e = a} \<union> the ` {e \<in> range (pt_walk (ASID s) (MEM s) (TTBR0 s)). \<not> is_fault e} = 
-            tlb_sat_no_flt_set s - {e \<in> tlb_sat_no_flt_set s. asid_entry e = a}")
+    apply (subgoal_tac "{e \<in> tlb_sat_set s. asid_entry e = a} \<inter> the ` {e \<in> range (pt_walk (ASID s) (MEM s) (TTBR0 s)). \<not> is_fault e} = {}")
+     apply (subgoal_tac "tlb_sat_set s - {e \<in> tlb_sat_set s. asid_entry e = a} \<union> the ` {e \<in> range (pt_walk (ASID s) (MEM s) (TTBR0 s)). \<not> is_fault e} = 
+            tlb_sat_set s - {e \<in> tlb_sat_set s. asid_entry e = a}")
       prefer 2
       apply blast
      apply clarsimp
-     apply (subgoal_tac " lookup (tlb_sat_no_flt_set s) (ASID s) (  b) = Hit x")
+     apply (subgoal_tac " lookup (tlb_sat_set s) (ASID s) (  b) = Hit x")
       apply blast
      apply (clarsimp simp: lookup_minus_hit_asid_hit)
     apply (clarsimp simp: asid_entry_set_inter)
@@ -234,21 +234,21 @@ lemma flush_asid_sat_no_flt_abs_refine':
   apply (rule conjI)
    prefer 2
    using lookup_miss_is_fault_intro lookup_miss_union_equal lookup_tlb_minus_asid_miss apply force
-   apply (subgoal_tac " lookup (tlb_sat_no_flt_set s) (ASID s) b = Hit x")
+   apply (subgoal_tac " lookup (tlb_sat_set s) (ASID s) b = Hit x")
      apply force
    apply (subgoal_tac "ASID s \<noteq> a")
    apply (simp add: lookup_minus_hit_asid_hit lookup_miss_is_fault_intro lookup_miss_union_equal)
   using lookup_miss_is_fault_intro lookup_miss_union_equal lookup_tlb_minus_asid_miss apply force
   apply (rule conjI)
-   apply (clarsimp simp: saturated_no_flt_def)
+   apply (clarsimp simp: saturated_def)
   apply (rule conjI)
    apply clarsimp
    apply (rule conjI)
     apply (clarsimp simp: snapshot_of_tlb_def)
      using asid_unequal_miss'' lookup_miss_union_equal lookup_tlb_minus_asid_miss apply force
    apply (clarsimp simp: snapshot_of_tlb_def)
-   apply (subgoal_tac "lookup (tlb_sat_no_flt_set s - {e \<in> tlb_sat_no_flt_set s. asid_entry e = a} \<union> 
-          the ` {e \<in> range (pt_walk (ASID s) (MEM s) (TTBR0 s)). \<not> is_fault e}) aa v = lookup (tlb_sat_no_flt_set s) aa  v")
+   apply (subgoal_tac "lookup (tlb_sat_set s - {e \<in> tlb_sat_set s. asid_entry e = a} \<union> 
+          the ` {e \<in> range (pt_walk (ASID s) (MEM s) (TTBR0 s)). \<not> is_fault e}) aa v = lookup (tlb_sat_set s) aa  v")
     apply clarsimp
    apply (subgoal_tac "asid_entry ` the ` {e \<in> range (pt_walk (ASID s) (MEM s) (TTBR0 s)). \<not> is_fault e} = {ASID s} \<or>
         asid_entry ` the ` {e \<in> range (pt_walk (ASID s) (MEM s) (TTBR0 s)). \<not> is_fault e} = {}")
@@ -277,26 +277,26 @@ lemma flush_varange_non_det_det_refine:
   apply (cases s, cases t , clarsimp simp: state.defs tlb_rel_def) 
   by blast
 
-lemma  flush_varange_det_sat_no_flt_refine:
-  "\<lbrakk> Flush_varange vset (s::tlb_det_state) = ((), s') ;  Flush_varange vset (t::tlb_sat_no_flt_state) = ((), t'); 
-         tlb_rel_sat_no_flt (typ_det_tlb s) (typ_sat_no_flt_tlb t) \<rbrakk> \<Longrightarrow> 
-                  tlb_rel_sat_no_flt (typ_det_tlb s') (typ_sat_no_flt_tlb t')"
-  apply (clarsimp simp: Flush_varange_tlb_det_state_ext_def Flush_varange_tlb_sat_no_flt_state_ext_def)
-  apply (clarsimp simp: tlb_rel_sat_no_flt_def saturated_no_flt_def )
+lemma  flush_varange_det_sat_refine:
+  "\<lbrakk> Flush_varange vset (s::tlb_det_state) = ((), s') ;  Flush_varange vset (t::tlb_sat_state) = ((), t'); 
+         tlb_rel_sat (typ_det_tlb s) (typ_sat_tlb t) \<rbrakk> \<Longrightarrow> 
+                  tlb_rel_sat (typ_det_tlb s') (typ_sat_tlb t')"
+  apply (clarsimp simp: Flush_varange_tlb_det_state_ext_def Flush_varange_tlb_sat_state_ext_def)
+  apply (clarsimp simp: tlb_rel_sat_def saturated_def )
   apply (cases s, cases t , clarsimp simp: state.defs)
   by blast
 
 lemma saturatd_lookup_hit_no_fault:
-  "\<lbrakk>saturated_no_flt (typ_sat_no_flt_tlb s);
-          lookup (tlb_sat_no_flt_set s) (ASID s) b = Hit x; \<not> is_fault (pt_walk (ASID s) (MEM s) (TTBR0 s) b)\<rbrakk>
+  "\<lbrakk>saturated (typ_sat_tlb s);
+          lookup (tlb_sat_set s) (ASID s) b = Hit x; \<not> is_fault (pt_walk (ASID s) (MEM s) (TTBR0 s) b)\<rbrakk>
                 \<Longrightarrow> x = the (pt_walk (ASID s) (MEM s) (TTBR0 s) b)"
-  apply (subgoal_tac "lookup (tlb_sat_no_flt_set s \<union> 
+  apply (subgoal_tac "lookup (tlb_sat_set s \<union> 
                               the ` {e \<in> range (pt_walk (ASID s) (MEM s) (TTBR0 s)). \<not> is_fault e}) (ASID s) (  b) = Hit x")
    prefer 2
    apply (drule sat_state_tlb', clarsimp simp: state.defs)
   apply (drule lookup_hit_miss_or_hit')
   apply (erule disjE)
-   apply (clarsimp simp: lookup_range_pt_walk_hit_no_flt)
+   apply (clarsimp simp: lookup_range_pt_walk_hit)
   apply (frule lookup_range_fault_pt_walk)
   apply (drule_tac x = "  b" in bspec; clarsimp simp: lookup_hit_entry_range)
   done
@@ -327,10 +327,10 @@ lemma  lookup_not_miss_varange:
 
 lemma lookup_not_miss_varange':
   "v \<in> vset\<Longrightarrow> 
-   lookup (tlb_sat_no_flt_set s - (\<Union>v\<in>vset. {e \<in> tlb_sat_no_flt_set s.   v \<in> entry_range e})) a (  v) =
+   lookup (tlb_sat_set s - (\<Union>v\<in>vset. {e \<in> tlb_sat_set s.   v \<in> entry_range e})) a (  v) =
                Miss"
-  apply (subgoal_tac "entry_set (tlb_sat_no_flt_set s - 
-              (\<Union>v\<in>vset. {e \<in> tlb_sat_no_flt_set s.   v \<in> entry_range e})) a (  v) = {}")
+  apply (subgoal_tac "entry_set (tlb_sat_set s - 
+              (\<Union>v\<in>vset. {e \<in> tlb_sat_set s.   v \<in> entry_range e})) a (  v) = {}")
    apply (clarsimp simp: lookup_def)
   by (clarsimp simp: entry_set_va_set a_va_set_def entry_range_asid_tags_def)
 
@@ -370,14 +370,14 @@ lemma  lookup_minus_hit':
 
 
 
-lemma flush_varange_sat_no_flt_abs_refine':
-  "\<lbrakk>Flush_varange vset (s::tlb_sat_no_flt_state) = ((), s') ;  Flush_varange vset (t::tlb_incon_state') = ((), t'); 
-             tlb_rel_abs' (typ_sat_no_flt_tlb s) (typ_incon' t) \<rbrakk> \<Longrightarrow> tlb_rel_abs' (typ_sat_no_flt_tlb s') (typ_incon' t')"
-  apply (clarsimp simp: Flush_varange_tlb_sat_no_flt_state_ext_def 
+lemma flush_varange_sat_abs_refine':
+  "\<lbrakk>Flush_varange vset (s::tlb_sat_state) = ((), s') ;  Flush_varange vset (t::tlb_incon_state') = ((), t'); 
+             tlb_rel_abs' (typ_sat_tlb s) (typ_incon' t) \<rbrakk> \<Longrightarrow> tlb_rel_abs' (typ_sat_tlb s') (typ_incon' t')"
+  apply (clarsimp simp: Flush_varange_tlb_sat_state_ext_def 
       Flush_varange_tlb_incon_state'_ext_def tlb_rel_abs'_def)
   apply (rule conjI)
    apply (cases s, cases t, clarsimp simp: state.defs)
-  apply (subgoal_tac "tlb_sat_no_flt_set s = tlb_sat_no_flt_set s \<union> 
+  apply (subgoal_tac "tlb_sat_set s = tlb_sat_set s \<union> 
                               the ` {e \<in> range (pt_walk (ASID s) (MEM s) (TTBR0 s)). \<not> is_fault e}")
    prefer 2
    apply (drule sat_state_tlb', clarsimp simp: state.defs)
@@ -387,7 +387,7 @@ lemma flush_varange_sat_no_flt_abs_refine':
     apply (clarsimp simp: asid_va_incon_def)
     apply (drule union_incon_cases1)
     apply (erule disjE)
-     apply (clarsimp simp: lookup_no_flt_range_pt_walk_not_incon')
+     apply (clarsimp simp: lookup_range_pt_walk_not_incon')
     apply (erule disjE)
      apply clarsimp
      apply (subgoal_tac "a = ASID s")
@@ -397,8 +397,8 @@ lemma flush_varange_sat_no_flt_abs_refine':
        apply (subgoal_tac "  b \<in> entry_range x")
         apply blast
        apply (clarsimp simp:lookup_hit_entry_range)
-      apply (subgoal_tac "lookup (tlb_sat_no_flt_set s) (ASID s) (  b) = Hit x  \<or> 
-                     lookup (tlb_sat_no_flt_set s ) (ASID s) (  b) = Incon")
+      apply (subgoal_tac "lookup (tlb_sat_set s) (ASID s) (  b) = Hit x  \<or> 
+                     lookup (tlb_sat_set s ) (ASID s) (  b) = Incon")
        apply (erule disjE)
         apply (subgoal_tac "x = the (pt_walk (ASID s) (MEM s) (TTBR0 s) xb)")
          apply clarsimp
@@ -415,21 +415,21 @@ lemma flush_varange_sat_no_flt_abs_refine':
      prefer 2
      apply (erule disjE)
       apply clarsimp
-      apply (clarsimp simp: lookup_no_flt_range_pt_walk_not_incon')
+      apply (clarsimp simp: lookup_range_pt_walk_not_incon')
      apply (erule disjE)
       apply clarsimp
-      apply (subgoal_tac " lookup (tlb_sat_no_flt_set s) a (  b) = Incon")
+      apply (subgoal_tac " lookup (tlb_sat_set s) a (  b) = Incon")
        apply (rule conjI)
         apply blast
-       apply (rule_tac tlb = "tlb_sat_no_flt_set s" and a = a in lookup_not_miss_varange, clarsimp)
+       apply (rule_tac tlb = "tlb_sat_set s" and a = a in lookup_not_miss_varange, clarsimp)
       apply (drule lookup_incon_minus, clarsimp)
      apply (erule disjE)
-      apply (clarsimp simp: lookup_no_flt_range_pt_walk_not_incon')
+      apply (clarsimp simp: lookup_range_pt_walk_not_incon')
      apply clarsimp
-     apply (subgoal_tac " lookup (tlb_sat_no_flt_set s) a (  b) = Incon")
+     apply (subgoal_tac " lookup (tlb_sat_set s) a (  b) = Incon")
       apply (rule conjI)
        apply blast
-      apply (rule_tac tlb = "tlb_sat_no_flt_set s" and a = a in lookup_not_miss_varange, clarsimp)
+      apply (rule_tac tlb = "tlb_sat_set s" and a = a in lookup_not_miss_varange, clarsimp)
      apply (drule lookup_incon_minus, clarsimp)
     prefer 2
     apply (clarsimp simp: asid_va_hit_incon_inter_def)
@@ -439,8 +439,8 @@ lemma flush_varange_sat_no_flt_abs_refine':
      apply (erule disjE)
       apply clarsimp
       apply (rule conjI)
-       apply (subgoal_tac "lookup (tlb_sat_no_flt_set s) (ASID s) (  b) = Hit x  \<or> 
-                     lookup (tlb_sat_no_flt_set s ) (ASID s) (  b) = Incon")
+       apply (subgoal_tac "lookup (tlb_sat_set s) (ASID s) (  b) = Hit x  \<or> 
+                     lookup (tlb_sat_set s ) (ASID s) (  b) = Incon")
         apply (erule disjE)
          prefer 2
          apply (clarsimp simp: asid_va_incon_def , blast)
@@ -448,7 +448,7 @@ lemma flush_varange_sat_no_flt_abs_refine':
          apply blast
         apply blast
        apply (drule lookup_hit_incon_minus, clarsimp) 
-      apply (rule_tac tlb = "tlb_sat_no_flt_set s" and a = "ASID s" in lookup_not_miss_varange, clarsimp)
+      apply (rule_tac tlb = "tlb_sat_set s" and a = "ASID s" in lookup_not_miss_varange, clarsimp)
      apply (erule disjE)
       apply clarsimp
       apply (frule lookup_range_fault_pt_walk)
@@ -461,8 +461,8 @@ lemma flush_varange_sat_no_flt_abs_refine':
      apply (drule lookup_hit_union_cases')
      apply (erule disjE)
       apply clarsimp
-      apply (subgoal_tac "lookup (tlb_sat_no_flt_set s) (ASID s) (  b) = Hit x  \<or> 
-                     lookup (tlb_sat_no_flt_set s ) (ASID s) (  b) = Incon")
+      apply (subgoal_tac "lookup (tlb_sat_set s) (ASID s) (  b) = Hit x  \<or> 
+                     lookup (tlb_sat_set s ) (ASID s) (  b) = Incon")
        apply (erule disjE)
         prefer 2
         apply (clarsimp simp: asid_va_incon_def , blast)
@@ -473,36 +473,36 @@ lemma flush_varange_sat_no_flt_abs_refine':
      apply (clarsimp simp: lookup_miss_is_fault_intro)
     prefer 3
     apply (rule conjI)
-     apply (clarsimp simp: saturated_no_flt_def)
+     apply (clarsimp simp: saturated_def)
     apply (rule conjI)
      apply clarsimp
      apply (rule conjI)
       apply (clarsimp simp: snapshot_of_tlb_def)
-      apply (subgoal_tac "lookup (tlb_sat_no_flt_set s - 
-                              (\<Union>v\<in>vset. {e \<in> tlb_sat_no_flt_set s.   v \<in> entry_range e}))  a (  v) =  Miss")
+      apply (subgoal_tac "lookup (tlb_sat_set s - 
+                              (\<Union>v\<in>vset. {e \<in> tlb_sat_set s.   v \<in> entry_range e}))  a (  v) =  Miss")
        apply (subgoal_tac "lookup ( the ` {e \<in> range (pt_walk (ASID s) (MEM s) (TTBR0 s)). \<not> is_fault e}) a (  v) = Miss")
         apply (rule lookup_miss_union_miss_miss; clarsimp)
-       apply (clarsimp simp: lookup_no_flt_range_pt_walk_asid_miss)
+       apply (clarsimp simp: lookup_range_pt_walk_asid_miss)
       apply (clarsimp simp: lookup_not_miss_varange')
      apply (clarsimp simp: snapshot_of_tlb_def)
-     apply (subgoal_tac "lookup (tlb_sat_no_flt_set s - (\<Union>v\<in>vset. {e \<in> tlb_sat_no_flt_set s.   v \<in> entry_range e}) \<union>
+     apply (subgoal_tac "lookup (tlb_sat_set s - (\<Union>v\<in>vset. {e \<in> tlb_sat_set s.   v \<in> entry_range e}) \<union>
                        the ` {e \<in> range (pt_walk (ASID s) (MEM s) (TTBR0 s)). \<not> is_fault e}) a (  v) = 
-             lookup (tlb_sat_no_flt_set s - (\<Union>v\<in>vset. {e \<in> tlb_sat_no_flt_set s.   v \<in> entry_range e}))  a (  v)")
+             lookup (tlb_sat_set s - (\<Union>v\<in>vset. {e \<in> tlb_sat_set s.   v \<in> entry_range e}))  a (  v)")
       apply (clarsimp)
-      apply (subgoal_tac " lookup (tlb_sat_no_flt_set s - (\<Union>v\<in>vset. {e \<in> tlb_sat_no_flt_set s.   v \<in> entry_range e})) a (  v) \<le>
-                                lookup (tlb_sat_no_flt_set s) a (  v)")
+      apply (subgoal_tac " lookup (tlb_sat_set s - (\<Union>v\<in>vset. {e \<in> tlb_sat_set s.   v \<in> entry_range e})) a (  v) \<le>
+                                lookup (tlb_sat_set s) a (  v)")
        apply (force simp add: less_eq_lookup_type)
       apply (rule tlb_mono)
       apply blast
      apply (rule lookup_miss_union_equal)
-     apply (clarsimp simp: lookup_no_flt_range_pt_walk_asid_miss)
+     apply (clarsimp simp: lookup_range_pt_walk_asid_miss)
     apply clarsimp
     apply blast
 proof -
   fix b :: vaddr and x :: tlb_entry
   assume a1: "is_fault (pt_walk (ASID s) (MEM s) (TTBR0 s) b)"
-  assume "lookup (tlb_sat_no_flt_set s - (\<Union>v\<in>vset. {e \<in> tlb_sat_no_flt_set s. v \<in> entry_range e}) \<union> the ` {e \<in> range (pt_walk (ASID s) (MEM s) (TTBR0 s)). \<not> is_fault e}) (ASID s) b = Hit x"
-  then have f2: "lookup (the ` {z \<in> range (pt_walk (ASID s) (MEM s) (TTBR0 s)). \<not> is_fault z}) (ASID s) b = Hit x \<or> lookup (tlb_sat_no_flt_set s - (\<Union>a\<in>vset. {t \<in> tlb_sat_no_flt_set s. a \<in> entry_range t})) (ASID s) b = Hit x"
+  assume "lookup (tlb_sat_set s - (\<Union>v\<in>vset. {e \<in> tlb_sat_set s. v \<in> entry_range e}) \<union> the ` {e \<in> range (pt_walk (ASID s) (MEM s) (TTBR0 s)). \<not> is_fault e}) (ASID s) b = Hit x"
+  then have f2: "lookup (the ` {z \<in> range (pt_walk (ASID s) (MEM s) (TTBR0 s)). \<not> is_fault z}) (ASID s) b = Hit x \<or> lookup (tlb_sat_set s - (\<Union>a\<in>vset. {t \<in> tlb_sat_set s. a \<in> entry_range t})) (ASID s) b = Hit x"
     using lookup_not_hit_false by blast
   have "lookup (the ` {z \<in> range (pt_walk (ASID s) (MEM s) (TTBR0 s)). \<not> is_fault z}) (ASID s) b \<noteq> Hit x"
     using a1 by (simp add: lookup_miss_is_fault_intro)
@@ -513,13 +513,13 @@ proof -
 next
   fix b :: vaddr and x :: tlb_entry and xb :: vaddr
   assume a1: "lookup (the ` {e \<in> range (pt_walk (ASID s) (MEM s) (TTBR0 s)). \<not> is_fault e}) (ASID s) b = Hit (the (pt_walk (ASID s) (MEM s) (TTBR0 s) xb))"
-  assume a2: "lookup (tlb_sat_no_flt_set s) (ASID s) b = Hit x"
-  assume a3: "saturated_no_flt (typ_sat_no_flt_tlb s)"
+  assume a2: "lookup (tlb_sat_set s) (ASID s) b = Hit x"
+  assume a3: "saturated (typ_sat_tlb s)"
   assume "x \<noteq> the (pt_walk (ASID s) (MEM s) (TTBR0 s) xb)"
   have "\<not> is_fault (pt_walk (ASID s) (MEM s) (TTBR0 s) b)"
     using a1 lookup_miss_is_fault_intro by force
   then show "x = the (pt_walk (ASID s) (MEM s) (TTBR0 s) xb)"
-    using a3 a2 a1 lookup_range_pt_walk_hit_no_flt saturatd_lookup_hit_no_fault by fastforce
+    using a3 a2 a1 lookup_range_pt_walk_hit saturatd_lookup_hit_no_fault by fastforce
 qed
 
 
@@ -542,12 +542,12 @@ lemma flush_ASIDvarange_non_det_det_refine:
   apply (cases s, cases t , clarsimp simp: state.defs tlb_rel_def) 
   by blast
 
-lemma  flush_ASIDvarange_det_sat_no_flt_refine:
-  "\<lbrakk> Flush_ASIDvarange a vset (s::tlb_det_state) = ((), s') ;  Flush_ASIDvarange a vset (t::tlb_sat_no_flt_state) = ((), t'); 
-         tlb_rel_sat_no_flt (typ_det_tlb s) (typ_sat_no_flt_tlb t) \<rbrakk> \<Longrightarrow> 
-                  tlb_rel_sat_no_flt (typ_det_tlb s') (typ_sat_no_flt_tlb t')"
-  apply (clarsimp simp: Flush_ASIDvarange_tlb_det_state_ext_def Flush_ASIDvarange_tlb_sat_no_flt_state_ext_def)
-  apply (clarsimp simp: tlb_rel_sat_no_flt_def saturated_no_flt_def)
+lemma  flush_ASIDvarange_det_sat_refine:
+  "\<lbrakk> Flush_ASIDvarange a vset (s::tlb_det_state) = ((), s') ;  Flush_ASIDvarange a vset (t::tlb_sat_state) = ((), t'); 
+         tlb_rel_sat (typ_det_tlb s) (typ_sat_tlb t) \<rbrakk> \<Longrightarrow> 
+                  tlb_rel_sat (typ_det_tlb s') (typ_sat_tlb t')"
+  apply (clarsimp simp: Flush_ASIDvarange_tlb_det_state_ext_def Flush_ASIDvarange_tlb_sat_state_ext_def)
+  apply (clarsimp simp: tlb_rel_sat_def saturated_def)
   apply (cases s, cases t , clarsimp simp: state.defs)
   by blast
 
@@ -555,24 +555,24 @@ lemma  flush_ASIDvarange_det_sat_no_flt_refine:
 
 lemma lookup_miss_diff_asid_varange:
   " a \<noteq> ASID s
-              \<Longrightarrow> lookup (\<Union>x\<in>{a} \<times> vset. case x of (a, v) \<Rightarrow> {e \<in> tlb_sat_no_flt_set s. (a,   v) \<in> entry_range_asid_tags e})
+              \<Longrightarrow> lookup (\<Union>x\<in>{a} \<times> vset. case x of (a, v) \<Rightarrow> {e \<in> tlb_sat_set s. (a,   v) \<in> entry_range_asid_tags e})
                    (ASID s) (  b) =
                   Miss"
- apply (subgoal_tac "entry_set (\<Union>x\<in>{a} \<times> vset. case x of (a, v) \<Rightarrow> {e \<in> tlb_sat_no_flt_set s. (a,   v) \<in> entry_range_asid_tags e})
+ apply (subgoal_tac "entry_set (\<Union>x\<in>{a} \<times> vset. case x of (a, v) \<Rightarrow> {e \<in> tlb_sat_set s. (a,   v) \<in> entry_range_asid_tags e})
                    (ASID s) (  b) = {}")
    apply (clarsimp simp: lookup_def)
   by (clarsimp simp: entry_set_va_set a_va_set_def entry_range_asid_tags_def)
 
 
 lemma lookup_asid_va_range_elem:
-  "lookup (\<Union>x\<in>{ASID s} \<times> vset. case x of (a, v) \<Rightarrow> {e \<in> tlb_sat_no_flt_set s. (a,   v) \<in> entry_range_asid_tags e}) (ASID s) (  b) = Hit x \<Longrightarrow>
-        b \<in> \<Union>(entry_range ` (\<Union>x\<in>{ASID s} \<times> vset. case x of (a, v) \<Rightarrow> {e \<in> tlb_sat_no_flt_set s. (a,   v) \<in> entry_range_asid_tags e}))"
+  "lookup (\<Union>x\<in>{ASID s} \<times> vset. case x of (a, v) \<Rightarrow> {e \<in> tlb_sat_set s. (a,   v) \<in> entry_range_asid_tags e}) (ASID s) (  b) = Hit x \<Longrightarrow>
+        b \<in> \<Union>(entry_range ` (\<Union>x\<in>{ASID s} \<times> vset. case x of (a, v) \<Rightarrow> {e \<in> tlb_sat_set s. (a,   v) \<in> entry_range_asid_tags e}))"
   apply (clarsimp simp: lookup_def  entry_set_def entry_range_asid_tags_def  split:if_split_asm)
   by force
 
 
 lemma  asidvset_elem_lookup_miss:
-  "b \<in> vset \<Longrightarrow>  lookup (tlb_sat_no_flt_set s - (\<Union>v\<in>vset. {e \<in> tlb_sat_no_flt_set s. (ASID s,   v) \<in> entry_range_asid_tags e}))
+  "b \<in> vset \<Longrightarrow>  lookup (tlb_sat_set s - (\<Union>v\<in>vset. {e \<in> tlb_sat_set s. (ASID s,   v) \<in> entry_range_asid_tags e}))
                 (ASID s) (  b) = Miss"
   apply (clarsimp simp: lookup_def entry_set_def entry_range_asid_tags_def)
   apply safe
@@ -580,7 +580,7 @@ lemma  asidvset_elem_lookup_miss:
 
 
 lemma   asidvset_elem_lookup_miss':
-  "b \<in> vset \<Longrightarrow>  lookup (tlb_sat_no_flt_set s - (\<Union>v\<in>vset. {e \<in> tlb_sat_no_flt_set s. (a,   v) \<in> entry_range_asid_tags e}))
+  "b \<in> vset \<Longrightarrow>  lookup (tlb_sat_set s - (\<Union>v\<in>vset. {e \<in> tlb_sat_set s. (a,   v) \<in> entry_range_asid_tags e}))
                 a (  b) = Miss"
   apply (clarsimp simp: lookup_def entry_set_def entry_range_asid_tags_def)
   apply safe
@@ -591,14 +591,14 @@ lemma  lookup_not_miss_asidvarange:
   apply (clarsimp simp: lookup_def entry_set_def entry_range_asid_tags_def split:if_split_asm) 
    by auto
 
-lemma flush_ASIDvarange_sat_no_flt_abs_refine':
-  "\<lbrakk>Flush_ASIDvarange a vset (s::tlb_sat_no_flt_state) = ((), s') ; Flush_ASIDvarange a vset (t::tlb_incon_state') = ((), t'); 
-             tlb_rel_abs' (typ_sat_no_flt_tlb s) (typ_incon' t) \<rbrakk> \<Longrightarrow> tlb_rel_abs' (typ_sat_no_flt_tlb s') (typ_incon' t')"
-  apply (clarsimp simp: Flush_ASIDvarange_tlb_sat_no_flt_state_ext_def 
+lemma flush_ASIDvarange_sat_abs_refine':
+  "\<lbrakk>Flush_ASIDvarange a vset (s::tlb_sat_state) = ((), s') ; Flush_ASIDvarange a vset (t::tlb_incon_state') = ((), t'); 
+             tlb_rel_abs' (typ_sat_tlb s) (typ_incon' t) \<rbrakk> \<Longrightarrow> tlb_rel_abs' (typ_sat_tlb s') (typ_incon' t')"
+  apply (clarsimp simp: Flush_ASIDvarange_tlb_sat_state_ext_def 
       Flush_ASIDvarange_tlb_incon_state'_ext_def tlb_rel_abs'_def)
   apply (rule conjI)
    apply (cases s, cases t, clarsimp simp: state.defs)
-  apply (subgoal_tac "tlb_sat_no_flt_set s = tlb_sat_no_flt_set s \<union> 
+  apply (subgoal_tac "tlb_sat_set s = tlb_sat_set s \<union> 
                               the ` {e \<in> range (pt_walk (ASID s) (MEM s) (TTBR0 s)). \<not> is_fault e}")
    prefer 2
    apply (drule sat_state_tlb', clarsimp simp: state.defs)
@@ -608,43 +608,43 @@ lemma flush_ASIDvarange_sat_no_flt_abs_refine':
     apply (clarsimp simp: asid_va_incon_def)
     apply (drule union_incon_cases1)
     apply (erule disjE)
-     apply (clarsimp simp: lookup_no_flt_range_pt_walk_not_incon')
+     apply (clarsimp simp: lookup_range_pt_walk_not_incon')
     apply (erule disjE)
      apply clarsimp
      apply (subgoal_tac "aa = ASID s")
       apply clarsimp
       apply (rule conjI)
-       apply (subgoal_tac "lookup (tlb_sat_no_flt_set s) (ASID s) (  b) = Hit x  \<or> 
-                     lookup (tlb_sat_no_flt_set s ) (ASID s) (  b) = Incon")
+       apply (subgoal_tac "lookup (tlb_sat_set s) (ASID s) (  b) = Hit x  \<or> 
+                     lookup (tlb_sat_set s ) (ASID s) (  b) = Incon")
         apply (erule disjE)
          prefer 2
          apply blast
         apply (subgoal_tac "\<not> is_fault (pt_walk (ASID s) (MEM s) (TTBR0 s) b)")
          prefer 2
   using lookup_miss_is_fault_intro apply force
-  using lookup_range_pt_walk_hit_no_flt saturatd_lookup_hit_no_fault apply fastforce
+  using lookup_range_pt_walk_hit saturatd_lookup_hit_no_fault apply fastforce
        apply (drule lookup_hit_incon_minus, clarsimp)
       apply (clarsimp simp: asidvset_elem_lookup_miss)
      apply (drule_tac t = "the ` {e \<in> range (pt_walk (ASID s) (MEM s) (TTBR0 s)). \<not> is_fault e}" in  lookup_hit_asid , clarsimp)
     apply (erule disjE)
      apply clarsimp
-     apply (clarsimp simp: lookup_no_flt_range_pt_walk_not_incon')
+     apply (clarsimp simp: lookup_range_pt_walk_not_incon')
     apply (erule disjE)
      apply clarsimp
-     apply (subgoal_tac " lookup (tlb_sat_no_flt_set s) aa (  b) = Incon")
+     apply (subgoal_tac " lookup (tlb_sat_set s) aa (  b) = Incon")
       apply (rule conjI)
        apply blast
       apply (rule impI)
-      apply (rule_tac tlb = "tlb_sat_no_flt_set s" and a = a in lookup_not_miss_asidvarange, clarsimp)
+      apply (rule_tac tlb = "tlb_sat_set s" and a = a in lookup_not_miss_asidvarange, clarsimp)
      apply (drule lookup_incon_minus, clarsimp)
     apply (erule disjE)
-     apply (clarsimp simp: lookup_no_flt_range_pt_walk_not_incon')
+     apply (clarsimp simp: lookup_range_pt_walk_not_incon')
     apply clarsimp
-    apply (subgoal_tac " lookup (tlb_sat_no_flt_set s) aa (  b) = Incon")
+    apply (subgoal_tac " lookup (tlb_sat_set s) aa (  b) = Incon")
      apply (rule conjI)
       apply blast
      apply (rule impI)
-     apply (rule_tac tlb = "tlb_sat_no_flt_set s" and a = a in lookup_not_miss_asidvarange, clarsimp)
+     apply (rule_tac tlb = "tlb_sat_set s" and a = a in lookup_not_miss_asidvarange, clarsimp)
     apply (drule lookup_incon_minus, clarsimp)
    apply (clarsimp simp: asid_va_hit_incon_inter_def)
    apply (rule conjI)
@@ -653,15 +653,15 @@ lemma flush_ASIDvarange_sat_no_flt_abs_refine':
     apply (erule disjE)
      apply clarsimp
      apply (rule conjI)
-      apply (subgoal_tac "lookup (tlb_sat_no_flt_set s) (ASID s) (  b) = Hit x  \<or> 
-                     lookup (tlb_sat_no_flt_set s ) (ASID s) (  b) = Incon")
+      apply (subgoal_tac "lookup (tlb_sat_set s) (ASID s) (  b) = Hit x  \<or> 
+                     lookup (tlb_sat_set s ) (ASID s) (  b) = Incon")
        apply (erule disjE)
         prefer 2
         apply (clarsimp simp: asid_va_incon_def , blast)
        apply force
       apply (drule lookup_hit_incon_minus, clarsimp)
      apply (rule impI)
-     apply (rule_tac tlb = "tlb_sat_no_flt_set s" and a = "ASID s" in lookup_not_miss_asidvarange, clarsimp)
+     apply (rule_tac tlb = "tlb_sat_set s" and a = "ASID s" in lookup_not_miss_asidvarange, clarsimp)
     apply (erule disjE)
      apply clarsimp
      apply (frule lookup_range_fault_pt_walk)
@@ -674,8 +674,8 @@ lemma flush_ASIDvarange_sat_no_flt_abs_refine':
     apply (drule lookup_hit_union_cases')
     apply (erule disjE)
      apply clarsimp
-     apply (subgoal_tac "lookup (tlb_sat_no_flt_set s) (ASID s) (  b) = Hit x  \<or> 
-                     lookup (tlb_sat_no_flt_set s ) (ASID s) (  b) = Incon")
+     apply (subgoal_tac "lookup (tlb_sat_set s) (ASID s) (  b) = Hit x  \<or> 
+                     lookup (tlb_sat_set s ) (ASID s) (  b) = Incon")
       apply (erule disjE)
        prefer 2
        apply (clarsimp simp: asid_va_incon_def , blast)
@@ -686,38 +686,38 @@ lemma flush_ASIDvarange_sat_no_flt_abs_refine':
     apply (clarsimp simp: lookup_miss_is_fault_intro)
    prefer 2
    apply (rule conjI)
-    apply (clarsimp simp: saturated_no_flt_def)
+    apply (clarsimp simp: saturated_def)
    apply (rule conjI)
     apply clarsimp
     apply (rule conjI)
      apply (clarsimp simp: snapshot_of_tlb_def)
-     apply (subgoal_tac "lookup (tlb_sat_no_flt_set s - 
-        (\<Union>v\<in>vset. {e \<in> tlb_sat_no_flt_set s. (a,   v) \<in> entry_range_asid_tags e}))  a (  v) =  Miss")
+     apply (subgoal_tac "lookup (tlb_sat_set s - 
+        (\<Union>v\<in>vset. {e \<in> tlb_sat_set s. (a,   v) \<in> entry_range_asid_tags e}))  a (  v) =  Miss")
       apply (subgoal_tac "lookup ( the `{e \<in> range (pt_walk (ASID s) (MEM s) (TTBR0 s)). \<not> is_fault e}) a (  v) = Miss")
        apply (rule lookup_miss_union_miss_miss ; clarsimp)
-      apply (clarsimp simp: lookup_no_flt_range_pt_walk_asid_miss)
+      apply (clarsimp simp: lookup_range_pt_walk_asid_miss)
      apply (clarsimp simp: asidvset_elem_lookup_miss')
     apply (clarsimp simp: snapshot_of_tlb_def)
-    apply (subgoal_tac "lookup (tlb_sat_no_flt_set s - (\<Union>v\<in>vset. {e \<in> tlb_sat_no_flt_set s. (a,   v) \<in> entry_range_asid_tags e}) \<union>
+    apply (subgoal_tac "lookup (tlb_sat_set s - (\<Union>v\<in>vset. {e \<in> tlb_sat_set s. (a,   v) \<in> entry_range_asid_tags e}) \<union>
                         the ` {e \<in> range (pt_walk (ASID s) (MEM s) (TTBR0 s)). \<not> is_fault e}) aa (  v) = 
-             lookup (tlb_sat_no_flt_set s - (\<Union>v\<in>vset. {e \<in> tlb_sat_no_flt_set s. (a,   v) \<in> entry_range_asid_tags e}))  aa (  v)")
+             lookup (tlb_sat_set s - (\<Union>v\<in>vset. {e \<in> tlb_sat_set s. (a,   v) \<in> entry_range_asid_tags e}))  aa (  v)")
      apply (clarsimp)
-     apply (subgoal_tac " lookup (tlb_sat_no_flt_set s - (\<Union>v\<in>vset. {e \<in> tlb_sat_no_flt_set s. (a,   v) \<in> entry_range_asid_tags e})) aa (  v) \<le>
-                                lookup (tlb_sat_no_flt_set s) aa (  v)")
+     apply (subgoal_tac " lookup (tlb_sat_set s - (\<Union>v\<in>vset. {e \<in> tlb_sat_set s. (a,   v) \<in> entry_range_asid_tags e})) aa (  v) \<le>
+                                lookup (tlb_sat_set s) aa (  v)")
       apply (force simp add: less_eq_lookup_type)
      apply (rule tlb_mono)
      apply blast
     apply (rule lookup_miss_union_equal)
-    apply (clarsimp simp: lookup_no_flt_range_pt_walk_asid_miss)
+    apply (clarsimp simp: lookup_range_pt_walk_asid_miss)
    apply clarsimp
    apply blast
 proof -
   fix b :: vaddr and x :: tlb_entry
-  assume a1: "lookup (tlb_sat_no_flt_set s - (\<Union>v\<in>vset. {e \<in> tlb_sat_no_flt_set s. (a, v) \<in> entry_range_asid_tags e}) \<union> the ` {e \<in> range (pt_walk (ASID s) (MEM s) (TTBR0 s)). \<not> is_fault e}) (ASID s) b = Hit x"
+  assume a1: "lookup (tlb_sat_set s - (\<Union>v\<in>vset. {e \<in> tlb_sat_set s. (a, v) \<in> entry_range_asid_tags e}) \<union> the ` {e \<in> range (pt_walk (ASID s) (MEM s) (TTBR0 s)). \<not> is_fault e}) (ASID s) b = Hit x"
   assume "is_fault (pt_walk (ASID s) (MEM s) (TTBR0 s) b)"
   moreover
   { assume "lookup (the ` {z \<in> range (pt_walk a (MEM s) (TTBR0 s)). \<not> is_fault z}) a b = Miss"
-    then have "(ASID s = a \<longrightarrow> b \<notin> vset) \<or> lookup (tlb_sat_no_flt_set s - (\<Union>aa\<in>vset. {t \<in> tlb_sat_no_flt_set s. (a, aa) \<in> entry_range_asid_tags t})) a b = Miss \<and> lookup (the ` {z \<in> range (pt_walk a (MEM s) (TTBR0 s)). \<not> is_fault z}) a b = Miss"
+    then have "(ASID s = a \<longrightarrow> b \<notin> vset) \<or> lookup (tlb_sat_set s - (\<Union>aa\<in>vset. {t \<in> tlb_sat_set s. (a, aa) \<in> entry_range_asid_tags t})) a b = Miss \<and> lookup (the ` {z \<in> range (pt_walk a (MEM s) (TTBR0 s)). \<not> is_fault z}) a b = Miss"
       using lookup_not_miss_asidvarange by blast
     then have "ASID s = a \<longrightarrow> b \<notin> vset"
       using a1 lookup_miss_union_miss_miss by force }
