MMU_ARMv7_Refinement_No_Fault/ARMv7_Update_TTBR0_Ref.thy
@@ -14,26 +14,26 @@ lemma update_ttbr0_non_det_det_refine:
    apply (cases s, cases t , clarsimp simp: state.defs tlb_rel_def) 
   by blast
 
-lemma  update_ttbr0_det_sat_no_flt_refine:
-  "\<lbrakk> update_TTBR0 r (s::tlb_det_state) = ((), s') ;  update_TTBR0 r (t::tlb_sat_no_flt_state) = ((), t'); 
-         tlb_rel_sat_no_flt (typ_det_tlb s) (typ_sat_no_flt_tlb t) \<rbrakk> \<Longrightarrow> 
-                  tlb_rel_sat_no_flt (typ_det_tlb s') (typ_sat_no_flt_tlb t')"
-  apply (clarsimp simp: update_TTBR0_tlb_det_state_ext_def update_TTBR0_tlb_sat_no_flt_state_ext_def)
-  apply (clarsimp simp: tlb_rel_sat_no_flt_def saturated_no_flt_def )
+lemma  update_ttbr0_det_sat_refine:
+  "\<lbrakk> update_TTBR0 r (s::tlb_det_state) = ((), s') ;  update_TTBR0 r (t::tlb_sat_state) = ((), t'); 
+         tlb_rel_sat (typ_det_tlb s) (typ_sat_tlb t) \<rbrakk> \<Longrightarrow> 
+                  tlb_rel_sat (typ_det_tlb s') (typ_sat_tlb t')"
+  apply (clarsimp simp: update_TTBR0_tlb_det_state_ext_def update_TTBR0_tlb_sat_state_ext_def)
+  apply (clarsimp simp: tlb_rel_sat_def saturated_def )
   apply (cases s, cases t , clarsimp simp: state.defs , force)
 done
 
 
-lemma lookup_no_flt_range_pt_walk_asid_miss:
+lemma lookup_range_pt_walk_asid_miss:
   "a \<noteq> a1 \<Longrightarrow> lookup (the ` {e \<in> range (pt_walk a mem ttbr0). \<not> is_fault e}) a1 va = Miss"
   apply (clarsimp simp: lookup_def entry_set_def entry_range_asid_tags_def)
   by force
 
-lemma lookup_no_flt_range_pt_walk_not_incon':
+lemma lookup_range_pt_walk_not_incon':
   "lookup (the ` {e \<in> range (pt_walk asid mem ttbr0). \<not> is_fault e}) asid1 va \<noteq> Incon"
   apply (case_tac "asid = asid1")
-   apply (clarsimp simp: lookup_no_flt_range_pt_walk_not_incon)
-  by (clarsimp simp: lookup_no_flt_range_pt_walk_asid_miss)
+   apply (clarsimp simp: lookup_range_pt_walk_not_incon)
+  by (clarsimp simp: lookup_range_pt_walk_asid_miss)
 
 
 
@@ -43,11 +43,11 @@ lemma lookup_miss_union:
   apply (clarsimp simp: lookup_def entry_set_def split: if_split_asm)
   by auto
        
-lemma sat_no_flt_miss_fault:
-  "\<lbrakk>saturated_no_flt (typ_sat_no_flt_tlb s);
-      lookup (tlb_sat_no_flt_set s) (ASID s) b = Miss\<rbrakk> \<Longrightarrow> is_fault (pt_walk (ASID s) (MEM s) (TTBR0 s) b)"
-  apply (subgoal_tac " lookup (tlb_sat_no_flt_set s  \<union> the ` {e \<in> range (pt_walk (ASID s) (MEM s) (TTBR0 s)). \<not> is_fault e}) (ASID s) (  b) = Miss")
-   apply (thin_tac " lookup (tlb_sat_no_flt_set s) (ASID s) (  b) = Miss")
+lemma sat_miss_fault:
+  "\<lbrakk>saturated (typ_sat_tlb s);
+      lookup (tlb_sat_set s) (ASID s) b = Miss\<rbrakk> \<Longrightarrow> is_fault (pt_walk (ASID s) (MEM s) (TTBR0 s) b)"
+  apply (subgoal_tac " lookup (tlb_sat_set s  \<union> the ` {e \<in> range (pt_walk (ASID s) (MEM s) (TTBR0 s)). \<not> is_fault e}) (ASID s) (  b) = Miss")
+   apply (thin_tac " lookup (tlb_sat_set s) (ASID s) (  b) = Miss")
    apply (drule lookup_miss_union)
    apply clarsimp
    apply (drule lookup_miss_is_fault)
@@ -62,16 +62,16 @@ lemma lookup_miss_snapshot:
   by (clarsimp simp: snapshot_of_tlb_def)
   
 
-lemma update_ttbr0_sat_no_flt_abs_refine':
-  "\<lbrakk> update_TTBR0 r (s::tlb_sat_no_flt_state) = ((), s') ;  update_TTBR0 r (t::tlb_incon_state') = ((), t'); 
-             tlb_rel_abs' (typ_sat_no_flt_tlb s) (typ_incon' t) \<rbrakk> \<Longrightarrow> 
-                     tlb_rel_abs' (typ_sat_no_flt_tlb s') (typ_incon' t')"
-  apply (clarsimp simp: update_TTBR0_tlb_sat_no_flt_state_ext_def update_TTBR0_tlb_incon_state'_ext_def tlb_rel_abs'_def)
+lemma update_ttbr0_sat_abs_refine':
+  "\<lbrakk> update_TTBR0 r (s::tlb_sat_state) = ((), s') ;  update_TTBR0 r (t::tlb_incon_state') = ((), t'); 
+             tlb_rel_abs' (typ_sat_tlb s) (typ_incon' t) \<rbrakk> \<Longrightarrow> 
+                     tlb_rel_abs' (typ_sat_tlb s') (typ_incon' t')"
+  apply (clarsimp simp: update_TTBR0_tlb_sat_state_ext_def update_TTBR0_tlb_incon_state'_ext_def tlb_rel_abs'_def)
   apply (subgoal_tac "ASID t = ASID s \<and> TTBR0 t = TTBR0 s \<and> MEM t = MEM s")
    prefer 2
-   apply (clarsimp simp: tlb_rel'_absD typ_sat_no_flt_tlb_def state.defs)
+   apply (clarsimp simp: tlb_rel'_absD typ_sat_tlb_def state.defs)
   apply (rule conjI)
-   apply (clarsimp simp: typ_sat_no_flt_tlb_def "state.defs")
+   apply (clarsimp simp: typ_sat_tlb_def "state.defs")
   apply (clarsimp simp: asid_va_incon_tlb_mem_def)
   apply (rule conjI)
    prefer 2
@@ -120,7 +120,7 @@ lemma update_ttbr0_sat_no_flt_abs_refine':
     prefer 2
     apply (drule union_incon_cases1)
     apply (erule disjE , force)
-    apply (clarsimp simp: lookup_no_flt_range_pt_walk_not_incon')
+    apply (clarsimp simp: lookup_range_pt_walk_not_incon')
     apply (erule disjE)
      apply (clarsimp simp: asid_unequal_miss'')
     apply (erule disjE)
@@ -137,23 +137,23 @@ lemma update_ttbr0_sat_no_flt_abs_refine':
     apply (drule union_incon_cases1 , clarsimp)
     apply (erule disjE, force)
     apply (erule disjE, clarsimp simp: asid_va_hit_incon_inter_def asid_va_hit_incon'_def asid_va_hit_incon''_def, force) 
-    apply (erule disjE, clarsimp simp: lookup_no_flt_range_pt_walk_not_incon)
+    apply (erule disjE, clarsimp simp: lookup_range_pt_walk_not_incon)
     apply (erule disjE, blast)
-    apply (erule disjE, clarsimp simp: lookup_no_flt_range_pt_walk_not_incon, blast)
+    apply (erule disjE, clarsimp simp: lookup_range_pt_walk_not_incon, blast)
    apply (erule disjE, clarsimp)
     apply (drule union_incon_cases1 , clarsimp)
     apply (erule disjE, force)
     apply (erule disjE, clarsimp simp: asid_va_hit_incon_inter_def asid_va_hit_incon'_def asid_va_hit_incon''_def, force) 
-    apply (erule disjE, clarsimp simp: lookup_no_flt_range_pt_walk_not_incon)
+    apply (erule disjE, clarsimp simp: lookup_range_pt_walk_not_incon)
     apply (erule disjE, blast)
-    apply (erule disjE, clarsimp simp: lookup_no_flt_range_pt_walk_not_incon, blast)
+    apply (erule disjE, clarsimp simp: lookup_range_pt_walk_not_incon, blast)
    apply (erule disjE, clarsimp)
     apply (drule union_incon_cases1 , clarsimp)
     apply (erule disjE, force)
     apply (erule disjE, clarsimp simp: asid_va_hit_incon_inter_def asid_va_hit_incon'_def asid_va_hit_incon''_def, force) 
-    apply (erule disjE, clarsimp simp: lookup_no_flt_range_pt_walk_not_incon)
+    apply (erule disjE, clarsimp simp: lookup_range_pt_walk_not_incon)
     apply (erule disjE, blast)
-    apply (erule disjE, clarsimp simp: lookup_no_flt_range_pt_walk_not_incon, blast)
+    apply (erule disjE, clarsimp simp: lookup_range_pt_walk_not_incon, blast)
    apply (drule union_incon_cases1 , clarsimp)
    apply (erule disjE, force)
    apply (erule disjE, clarsimp)
@@ -162,15 +162,15 @@ lemma update_ttbr0_sat_no_flt_abs_refine':
      apply force
     apply (frule lookup_range_fault_pt_walk)
     apply (drule_tac x = b in bspec, simp add: lookup_hit_entry_range, simp)
-   apply (erule disjE, clarsimp simp: lookup_no_flt_range_pt_walk_not_incon)
+   apply (erule disjE, clarsimp simp: lookup_range_pt_walk_not_incon)
    apply (erule disjE, blast)
-   apply (erule disjE, clarsimp simp: lookup_no_flt_range_pt_walk_not_incon, blast)
+   apply (erule disjE, clarsimp simp: lookup_range_pt_walk_not_incon, blast)
   apply (rule conjI)
-   apply (clarsimp simp:  saturated_no_flt_def)
+   apply (clarsimp simp:  saturated_def)
   apply (rule conjI)
    apply (clarsimp)
-   apply (subgoal_tac "snapshot_of_tlb (tlb_sat_no_flt_set s \<union> the `{e \<in> range (pt_walk (ASID s) (MEM s) r). \<not> is_fault e}) a v =
-                             snapshot_of_tlb  (tlb_sat_no_flt_set s) a v")
+   apply (subgoal_tac "snapshot_of_tlb (tlb_sat_set s \<union> the `{e \<in> range (pt_walk (ASID s) (MEM s) r). \<not> is_fault e}) a v =
+                             snapshot_of_tlb  (tlb_sat_set s) a v")
     apply clarsimp
    apply (rule lookup_miss_snapshot)
    apply (clarsimp simp: asid_unequal_miss'')
@@ -180,7 +180,7 @@ lemma update_ttbr0_sat_no_flt_abs_refine':
 
 
 
-lemma update_ttbr0_sat_no_flt_abs_refine'2:
+lemma update_ttbr0_sat_abs_refine'2:
   "\<lbrakk> update_TTBR0 r (s::tlb_incon_state') = ((), s') ;  update_TTBR0 r (t::tlb_incon_state) = ((), t'); 
              refine_rel (typ_incon' s) (typ_incon'2 t) \<rbrakk> \<Longrightarrow> 
                      refine_rel (typ_incon' s') (typ_incon'2 t')"
@@ -189,7 +189,7 @@ lemma update_ttbr0_sat_no_flt_abs_refine'2:
    prefer 2
    apply (clarsimp simp: typ_incon'2_def typ_incon'_def state.defs) 
   apply (rule conjI)
-   apply (clarsimp simp: typ_sat_no_flt_tlb_def "state.defs")
+   apply (clarsimp simp: typ_sat_tlb_def "state.defs")
   apply (rule conjI)
    apply clarsimp
    apply (drule_tac x = a in spec)
